refactoring: spill_live -> reconstr_live, new definitions, progress on new proof

theories/Spilling/DoSpill.v
@@ -5,10 +5,8 @@ Require Import SimI Spilling SpillUtil.
 
 Definition slot_lift_params
            (slot : var -> var)
-           (Z : params)
-           (rm : set var * set var)
-  :=
-    elements (of_list Z ∩ fst rm ∪ map slot (of_list Z ∩ snd rm))
+           (M : set var)
+  := (fun z => if [z ∈ M] then slot z else z)
 .
 
 
@@ -25,134 +23,594 @@ Proof.
 Qed.
 
 
-
-Definition do_spill' (slot : var -> var) (do_spill : forall
-                         (s : stmt)
-                         (sl0 : ann (set var * set var * option(list(set var * set var)))),
-                         stmt) s rm := fix f sl n {struct n} :=
-  let Sp := fst (fst (getAnn sl)) in
-  let L  := snd (fst (getAnn sl)) in
-  match n with
-  | 0 =>
-    match s,sl with
-    | stmtLet x e s, ann1 _ sl_s
-      => stmtLet x e (do_spill s sl_s)
-    | stmtIf e s t, ann2 _ sl_s sl_t
-      => stmtIf e (do_spill s sl_s) (do_spill t sl_t)
-    | stmtFun F t, annF (_,_,Some rms) sl_F sl_t
-      => stmtFun
-          ((fun Zs sls_rm
-            => let (sl_s,rm) := sls_rm
-                               : ann (set var * set var * option (list (set var * set var)))
-                                 * (set var * set var) in
-              (slot_lift_params slot (fst Zs) rm, do_spill (snd Zs) sl_s))
-             ⊜ F
-             ((fun sl_s rm => (sl_s,rm)) ⊜ sl_F rms))
-          (do_spill t sl_t)
-
-    | _,_
-      => s
-    end
-
-  | S n =>
-
-    if
-      [cardinal Sp = 0]
-    then
-      if
-        [cardinal L = 0]
-      then
-        match s,sl with
-        | stmtLet x e s, ann1 _ sl_s
-          => stmtLet x e (do_spill s sl_s)
-        | stmtIf e s t, ann2 _ sl_s sl_t
-          => stmtIf e (do_spill s sl_s) (do_spill t sl_t)
-        | stmtFun F t, annF (_,_,Some rms) sl_F sl_t
-          => stmtFun
-              ((fun Zs sls_rm
-                => let (sl_s,rm) := sls_rm
-                                   : ann (set var * set var * option (list (set var * set var)))
-                                     * (set var * set var) in
-                  (slot_lift_params slot (fst Zs) rm, do_spill (snd Zs) sl_s))
-                 ⊜ F
-                 ((fun sl_s rm => (sl_s,rm)) ⊜ sl_F rms))
-              (do_spill t sl_t)
-
-        | _,_
-          => s
-        end
-
-      else
-        let x := hd 0 (elements L) in
-        let L':= of_list (tl (elements L)) in
-        stmtLet x (Operation (Var (slot x))) (f (setTopAnn sl (Sp,L',rm)) n)
-
-    else
-      let x  := hd 0 (elements Sp) in
-      let Sp':= of_list (tl (elements Sp)) in
-      stmtLet (slot x) (Operation (Var x)) (f (setTopAnn sl (Sp',L,rm)) n)
-  end
-.
-
-Fixpoint do_spill
-         (slot : var -> var)
-         (s : stmt)
-         (sl0 : ann (set var * set var * option(list(set var * set var))))
-         {struct s}
-  : stmt :=
-  let Sp0 := fst (fst (getAnn sl0)) in
-  let L0  := snd (fst (getAnn sl0)) in
-  let rm  := snd (getAnn sl0) in
-  do_spill' slot (do_spill slot) s rm sl0 (cardinal Sp0 + cardinal L0)
+Definition slot_lift_args
+           (slot : var -> var)
+           (M : set var)
+  : op -> op
+  := (fun y => match y with
+            | Var v => if [v ∈ M] then Var (slot v) else Var v
+            | _ => y
+            end)
 .
 
 
+Definition write_spills
+           (slot : var -> var)
+           (Z : params)
+           (s : stmt)
+  : stmt
+  := fold_right (fun x s => stmtLet (slot x) (Operation (Var x)) s) s Z
+.
 
-Lemma do_spill_empty
+Definition write_loads
+           (slot : var -> var)
+           (Z : params)
+           (s : stmt)
+  : stmt
+  := fold_right (fun x s => stmtLet x (Operation (Var (slot x))) s) s Z
+.
+
+
+Lemma write_spills_empty
       (slot : var -> var)
       (s : stmt)
-      (sl : ann (set var * set var * option (list (set var * set var))))
   :
-    Empty (fst (fst (getAnn sl)))
-    -> Empty (snd (fst (getAnn sl)))
-    -> do_spill slot s sl
-      =
-
-      match s,sl with
-     | stmtLet x e s, ann1 _ sl_s
-       => stmtLet x e (do_spill slot s sl_s)
-     | stmtIf e s t, ann2 _ sl_s sl_t
-       => stmtIf e (do_spill slot s sl_s) (do_spill slot t sl_t)
-     | stmtFun F t, annF (_,_,Some rms) sl_F sl_t
-       => stmtFun
-           ((fun Zs sls_rm
-             => let (sl_s,rm) := sls_rm
-                                : ann (set var * set var * option (list (set var * set var)))
-                                  * (set var * set var) in
-               (slot_lift_params slot (fst Zs) rm, do_spill slot (snd Zs) sl_s))
-              ⊜ F
-              ((fun sl_s rm => (sl_s,rm)) ⊜ sl_F rms))
-           (do_spill slot t sl_t)
-
-     | _,_
-       => s
-      end.
+    write_spills slot nil s = s
+.
 Proof.
-  intros Empty_Sp Empty_L.
-  remember (fst (fst (getAnn sl))) as Sp.
-  remember (snd (fst (getAnn sl))) as L.
-  assert (cardinal Sp = 0) as zero_Sp.
-  { apply cardinal_Empty. eauto. }
-  assert (cardinal L = 0) as zero_L.
-  { apply cardinal_Empty. eauto. }
-  induction sl, s; simpl in *; rewrite <- HeqSp; rewrite <- HeqL;
-    simpl; rewrite zero_Sp; rewrite zero_L; simpl; eauto.
+  simpl.
+  reflexivity.
+Qed.
+
+
+Lemma write_loads_empty
+      (slot : var -> var)
+      (s : stmt)
+  :
+    write_loads slot nil s = s
+.
+Proof.
+  simpl.
+  reflexivity.
+Qed.
+
+
+Lemma write_spills_s
+      (slot : var -> var)
+      (xs : list var)
+      (x : var)
+      (s : stmt)
+  :
+    write_spills slot (x::xs) s
+    = stmtLet (slot x) (Operation (Var x)) (write_spills slot xs s)
+.
+Proof.
+  simpl.
+  reflexivity.
 Qed.
 
 
 
 
+Lemma write_loads_s
+      (slot : var -> var)
+      (xs : list var)
+      (x : var)
+      (s : stmt)
+  :
+    write_loads slot (x::xs) s
+    = stmtLet x (Operation (Var (slot x))) (write_loads slot xs s)
+.
+Proof.
+  simpl.
+  reflexivity.
+Qed.
 
+
+
+
+Definition do_spill_rec
+           (slot : var -> var)
+           (M : set var)
+           (s : stmt)
+           (sl : spilling)
+           (do_spill' : forall (s' : stmt)
+                           (sl' : spilling),
+                            stmt)
+  : stmt
+  :=
+    match s,sl with
+    | stmtLet x e s, ann1 _ sl1
+      => stmtLet x e (do_spill' s sl1)
+
+    | stmtIf e s1 s2, ann2 _ sl1 sl2
+      => stmtIf e (do_spill' s1 sl1) (do_spill' s2 sl2)
+
+    | stmtFun F t, annF (_,_,Some rms) sl_F sl_t
+      => stmtFun
+          ((fun pf sf => (pf,sf))
+             ⊜ ((fun (Zs : params * stmt) (rm : set var * set var)
+                 => slot_lift_params slot (snd rm) ⊝ (fst Zs)) ⊜ F rms)
+             ((fun (Zs : params * stmt) (sl_s : spilling)
+               => do_spill' (snd Zs) sl_s) ⊜ F sl_F)
+          )
+          (do_spill' t sl_t)
+
+    | stmtApp f Y, ann0 _
+      => stmtApp f ((slot_lift_args slot M) ⊝ Y)
+
+    | _,_
+      => s
+    end
+.
+
+
+
+(* this algorithm prefers variables in the memory in function applications *)
+Fixpoint do_spill
+           (slot : var -> var)
+           (M : set var)
+           (s : stmt)
+           (sl : spilling)
+  : stmt
+  :=
+    write_spills slot (elements (getSp sl)) (
+        write_loads slot (elements (getL sl)) (
+            let do_spill' := do_spill slot (getSp sl ∪ M) in
+            do_spill_rec slot (getSp sl ∪ M) s sl do_spill'
+        )
+     )
+.
+
+(*
+Fixpoint do_spill
+           (slot : var -> var)
+           (M : set var)
+           (s : stmt)
+           (sl : spilling)
+  : stmt
+  :=
+    write_spills slot (elements (getSp sl)) (
+        write_loads slot (elements (getL sl)) (
+            let do_spill' := do_spill slot (getSp sl ∪ M) in
+            match s,sl with
+            | stmtLet x e s, ann1 _ sl1
+              => stmtLet x e (do_spill' s sl1)
+
+            | stmtIf e s1 s2, ann2 _ sl1 sl2
+              => stmtIf e (do_spill' s1 sl1) (do_spill' s2 sl2)
+
+            | stmtFun F t, annF (_,_,Some rms) sl_F sl_t
+              => stmtFun
+                  ((fun pf sf => (pf,sf))
+                     ⊜ ((fun (Zs : params * stmt) (rm : set var * set var)
+                         => slot_lift_params slot (snd rm) ⊝ (fst Zs)) ⊜ F rms)
+                     ((fun (Zs : params * stmt) (sl_s : spilling)
+                       => do_spill' (snd Zs) sl_s) ⊜ F sl_F)
+                  )
+                  (do_spill' t sl_t)
+
+            | stmtApp f Y, ann0 _
+              => stmtApp f ((slot_lift_args slot M) ⊝ Y)
+
+            | _,_
+              => s
+            end
+        )
+     )
+.
+ *)
+
+
+Lemma count_zero_Empty_Sp
+      (sl : spilling)
+  :
+    count sl = 0
+    -> Empty (getSp sl)
+.
+Proof.
+  intro count_zero.
+  apply cardinal_Empty.
+  unfold count in count_zero.
+  omega.
+Qed.
+
+Lemma count_zero_cardinal_Sp
+      (sl : spilling)
+  :
+    count sl = 0
+    -> cardinal (getSp sl) = 0
+.
+Proof.
+  intro count_zero.
+  unfold count in count_zero.
+  omega.
+Qed.
+
+
+
+
+Lemma count_zero_cardinal_L
+      (sl : spilling)
+  :
+    count sl = 0
+    -> cardinal (getL sl) = 0
+.
+Proof.
+  intro count_zero.
+  unfold count in count_zero.
+  omega.
+Qed.
+
+
+Lemma count_zero_Empty_L
+      (sl : spilling)
+  :
+    count sl = 0
+    -> Empty (getL sl)
+.
+Proof.
+  intro count_zero.
+  apply cardinal_Empty.
+  unfold count in count_zero.
+  omega.
+Qed.
+
+
+Lemma Empty_Sp_L_count_zero
+      (sl : spilling)
+  :
+    Empty (getSp sl)
+    -> Empty (getL sl)
+    -> count sl = 0
+.
+Proof.
+  intros Empty_Sp Empty_L.
+  apply cardinal_Empty in Empty_Sp.
+  apply cardinal_Empty in Empty_L.
+  unfold count.
+  omega.
+Qed.
+
+
+
+Lemma slot_lift_args_Equal_M
+      (slot : var -> var)
+      (M M' : set var)
+      (y y' : op)
+  :
+    M [=] M'
+    -> y === y'
+    -> slot_lift_args slot M y = slot_lift_args slot M' y'
+.
+Proof.
+  intros eq_M eq_y.
+  destruct y;
+    destruct y';
+    isabsurd;
+    simpl;
+    eauto.
+  inv eq_y.
+  decide (v0 ∈ M).
+  - rewrite eq_M in i.
+    decide (v0 ∈ M').
+    + reflexivity.
+    + contradiction.
+  - rewrite eq_M in n.
+    decide (v0 ∈ M').
+    + contradiction.
+    + reflexivity.
+Qed.
+
+
+Lemma slot_lift_args_Equal_M_Y
+      (slot : var -> var)
+      (M M' : set var)
+      (Y Y' : args)
+  :
+    M [=] M'
+    -> Y === Y'
+    -> slot_lift_args slot M ⊝ Y = slot_lift_args slot M' ⊝ Y'
+.
+Proof.
+  intros eq_M eq_Y.
+  general induction Y;
+    inv eq_Y;
+    simpl; eauto.
+  erewrite slot_lift_args_Equal_M; eauto.
+  f_equal.
+  apply IHY; eauto.
+Qed.
+
+
+Lemma do_spill_rec_Equal_M
+      (slot : var -> var)
+      (M M' : set var)
+      (s : stmt)
+      (sl : spilling)
+  :
+    M [=] M'
+    -> do_spill_rec slot M s sl = do_spill_rec slot M' s sl
+.
+Proof.
+  intro eq_M.
+  destruct s; simpl; eauto.
+  destruct sl; simpl; eauto.
+  unfold do_spill_rec.
+  enough (slot_lift_args slot M ⊝ Y = slot_lift_args slot M' ⊝ Y) as H.
+  {
+    rewrite H.
+    reflexivity.
+  }
+  apply slot_lift_args_Equal_M_Y; eauto.
+Qed.
+
+
+Lemma do_spill_Equal_M
+      (slot : var -> var)
+      (M M' : ⦃ var ⦄)
+      (s : stmt)
+      (sl : spilling)
+  :
+    M [=] M'
+    -> do_spill slot M s sl = do_spill slot M' s sl
+.
+Proof.
+  intros eq_M.
+  general induction s;
+    simpl;
+    do 2 f_equal;
+    destruct sl;
+    eauto.
+  - rewrite IHs with (M':= getSp (ann1 a sl) ∪ M');
+      [ | rewrite eq_M ] ; eauto.
+  - erewrite IHs1 with (M':= getSp (ann2 a sl1 sl2) ∪ M');
+      [ | rewrite eq_M ] ; eauto.
+    erewrite IHs2 with (M':= getSp (ann2 a sl1 sl2) ∪ M');
+      [ | rewrite eq_M ] ; eauto.
+  - erewrite slot_lift_args_Equal_M_Y; eauto.
+    rewrite eq_M.
+    reflexivity.
+  - destruct a;
+      destruct p;
+      destruct o;
+      eauto.
+    rewrite IHs with (M':= getSp (annF (s0,s1,⎣l⎦) sa sl) ∪ M');
+      [ | rewrite eq_M ] ; eauto.
+    assert (((fun (Zs : params * stmt) (sl_s : spilling) =>
+                do_spill slot (getSp annF (s0, s1, ⎣ l ⎦) sa sl ∪ M) (snd Zs) sl_s) ⊜ F sa)
+           = (fun (Zs : params * stmt) (sl_s : spilling) =>
+        do_spill slot (getSp annF (s0, s1, ⎣ l ⎦) sa sl ∪ M') (snd Zs) sl_s) ⊜ F sa).
+    { admit. }
+    rewrite H.
+    reflexivity.
+Admitted.
+
+Lemma do_spill_rec_do_spill_Equal_M
+      (slot : var -> var)
+      (M M' : ⦃var⦄)
+      (s : stmt)
+      (sl : spilling)
+  :
+    M [=] M'
+    -> do_spill_rec slot M s sl (do_spill slot M)
+      = do_spill_rec slot M' s sl (do_spill slot M')
+.
+Admitted.
+(*
+Lemma do_spill_rec_do_spill_Equal_M
+      (slot : var -> var)
+      (M M' : ⦃var⦄)
+      (s : stmt)
+      (sl : spilling)
+      (do_spill' : forall (M0 : ⦃var⦄)
+                      (s0 : stmt)
+                      (sl0 : spilling),
+          stmt)
+  :
+    M [=] M'
+    -> do_spill' M = do_spill' M'
+    -> do_spill_rec slot M s sl (do_spill' M)
+      = do_spill_rec slot M' s sl (do_spill' M')
+.
+Proof.
+  intros eq_M.
+  general induction s;
+    simpl; eauto.
+  erewrite slot_lift_args_Equal_M_Y;
+    eauto.
+Qed.
+
+
+
+Lemma do_spill_Equal_M
+          (slot : var -> var)
+          (M M' : set var)
+          (s : stmt)
+          (sl : spilling)
+  :
+    M [=] M'
+    -> (forall M0 M0', M0 [=] M0'
+                 -> do_spill_rec slot M0 s sl (do_spill slot M0)
+                   = do_spill_rec slot M0' s sl (do_spill slot M0'))
+    -> do_spill slot M s sl
+      = do_spill slot M' s sl
+.
+Proof.
+  intros eq_M eq_dsr.
+  general induction s;
+    unfold do_spill;
+    f_equal;
+    f_equal;
+    destruct sl;
+    eauto;
+    apply eq_dsr;
+    rewrite eq_M;
+    reflexivity.
+Qed.
+*)
+(*
+Lemma do_spill_rec_Equal_M'
+      (slot : var -> var)
+      (M M' : ⦃ var ⦄)
+      (s : stmt)
+      (sl : spilling)
+  :
+    M [=] M'
+    -> do_spill_rec slot M s sl (do_spill slot M)
+      = do_spill_rec slot M' s sl (do_spill slot M')
+.
+Proof.
+  intros eq_M.
+  general induction s.
+    simpl; eauto.
+  - destruct sl; eauto.
+    erewrite do_spill_Equal_M; eauto.
+  - admit.
+  - admit.
+  - destruct sl; eauto.
+    destruct a;
+      destruct p;
+      destruct o;
+      eauto.
+    erewrite do_spill_Equal_M; eauto.
+    replace ((fun (Zs : params * stmt) (sl_s : spilling) => do_spill slot M (snd Zs) sl_s) ⊜ F sa)
+    with ((fun (Zs : params * stmt) (sl_s : spilling) => do_spill slot M' (snd Zs) sl_s) ⊜ F sa).
+    + reflexivity.
+    + f_equal.
+      extensionality ps'.
+      extensionality sl'.
+      symmetry.
+      eapply do_spill_Equal_M; eauto.
+      intros.
+      apply do_spill_rec_do_spill_Equal_M.
+
+uecouiaeou
+*)
+
+Lemma do_spill_rec_s
+      (slot : var -> var)
+      (M Sp' L': ⦃ var ⦄)
+      (s : stmt)
+      (sl : spilling)
+  :
+    do_spill_rec slot M s sl
+    = do_spill_rec slot M s (setTopAnn sl (Sp',L',snd (getAnn sl)))
+.
+Proof.
+  destruct s, sl;
+    simpl;
+    unfold do_spill_rec;
+    try reflexivity.
+  destruct a;
+    destruct p;
+    destruct o;
+    eauto.
+Qed.
+
+Lemma do_spill_empty
+      (slot : var -> var)
+      (M : set var)
+      (s : stmt)
+      (sl : spilling)
+  :
+    count sl = 0
+    -> do_spill slot M s sl
+      = do_spill_rec slot M s sl (do_spill slot M)
+.
+Proof.
+  intros count_zero.
+  apply count_zero_Empty_Sp in count_zero as Empty_Sp.
+  apply count_zero_Empty_L  in count_zero as Empty_L.
+  unfold do_spill.
+  rewrite elements_Empty in Empty_Sp.
+  rewrite elements_Empty in Empty_L.
+  assert (getSp sl ∪ M [=] M) as H.
+  {
+    apply elements_nil_eset in Empty_Sp.
+    rewrite Empty_Sp.
+    cset_tac.
+  }
+  induction s;
+    rewrite Empty_Sp;
+    rewrite Empty_L;
+    rewrite write_spills_empty;
+    rewrite write_loads_empty;
+    fold do_spill;
+    apply do_spill_rec_do_spill_Equal_M; (* !! this is unproven !! *)
+    rewrite H;
+    reflexivity.
+Qed.
+
+
+
+Lemma do_spill_extract_writes
+      (slot : var -> var)
+      (M : ⦃ var ⦄)
+      (s : stmt)
+      (sl : spilling)
+  :
+    do_spill slot M s sl
+    = write_spills slot (elements (getSp sl))
+                   (write_loads slot (elements (getL sl))
+                                (do_spill slot (getSp sl ∪ M) s (setTopAnn sl (∅,∅,snd (getAnn sl)))))
+.
+Proof.
+  symmetry.
+  rewrite do_spill_empty. (* !! this uses an unproven lemma !! *)
+  - rewrite do_spill_rec_s with (Sp':=∅) (L':=∅).
+    rewrite setTopAnn_setTopAnn.
+    destruct s,sl;
+      simpl; eauto.
+    do 2 f_equal.
+    destruct a.
+    simpl.
+    destruct o;
+      destruct p;
+      reflexivity.
+  - unfold count.
+    rewrite getAnn_setTopAnn.
+    simpl.
+    eauto.
+Qed.
+
+
+
+Lemma do_spill_sub_empty_invariant
+      (slot : var -> var)
+      (M Sp' L': ⦃ var ⦄)
+      (s : stmt)
+      (sl : spilling)
+  :
+    count sl = 0
+    -> Sp' [=] ∅
+    -> L' [=] ∅
+    ->  do_spill slot M s sl
+       = do_spill slot M s (setTopAnn sl (Sp',L',snd (getAnn sl)))
+.
+Proof.
+  intros count_zero Sp_empty L_empty.
+  rewrite do_spill_empty; eauto. (* !! this uses an unproven lemma !! *)
+  rewrite do_spill_empty;
+    swap 1 2.
+  {
+    unfold count.
+    rewrite getAnn_setTopAnn.
+    simpl.
+    rewrite Sp_empty.
+    rewrite L_empty.
+    eauto.
+  }
+  destruct s, sl;
+    simpl; eauto.
+  destruct a;
+    destruct p;
+    destruct o;
+    simpl; eauto.
+Qed.
+
+
+(*
 Lemma do_spill_Sp
       (slot : var -> var)
       (s : stmt)
@@ -195,16 +653,12 @@ Qed.
 Lemma do_spill_L
       (slot : var -> var)
       (s : stmt)
-      (sl : ann (set var * set var * option (list (set var * set var))))
+      (sl : spilling)
   :
-    let Sp := fst (fst (getAnn sl)) in
-    let L  := snd (fst (getAnn sl)) in
-    let x  := hd 0 (elements L) in
-    let L' := of_list (tl (elements L)) in
-    Empty Sp
-    -> ~ Empty L
+    cardinal (getSp sl) = 0
+    -> cardinal (getL sl) > 0
     -> do_spill slot s sl
-      = stmtLet x
+      = write_loads
                 (Operation (Var (slot x)))
                 (do_spill slot s (setTopAnn sl (Sp,L',snd (getAnn sl))))
 .
@@ -237,28 +691,17 @@ Proof.
 Qed.
 
 
-Lemma do_spill_empty_invariant
-      (slot : var -> var)
-      (s : stmt)
-      (Sp' L' : set var)
-      (sl sl' : ann (set var * set var * option ( list (set var * set var))))
-  :
-    sl' = setTopAnn sl (Sp',L',snd (getAnn sl))
-    -> Empty (fst (fst (getAnn sl)))
-    -> Empty (snd (fst (getAnn sl)))
-    -> Empty Sp'
-    -> Empty L'
-    -> do_spill slot s sl = do_spill slot s sl'
-.
-Proof.
-  intros top_sl' Empty_Sp Empty_L Empty_Sp' Empty_L'.
-  rewrite top_sl'.
-  rewrite do_spill_empty;
-    try rewrite getAnn_setTopAnn; eauto.
-  rewrite do_spill_empty;
-    try rewrite getAnn_setTopAnn; eauto.
-  unfold setTopAnn.
-  destruct sl; eauto.
-  destruct a; destruct p.
-  destruct s; eauto.
-Qed.
+
+
+
+
+
+
+
+
+
+
+
+
+
+*)
