theories/Spilling/DoSpillRm.v
@@ -1,63 +1,136 @@
 Require Import List Map Env AllInRel Exp AppExpFree.
 Require Import IL Annotation InRel AutoIndTac Liveness LabelsDefined.
-Require Import SpillUtil.
+Require Import Spilling SpillUtil.
+
+Set Implicit Arguments.
 
 
-
-
-
-Fixpoint do_spill_rm'
-         (slot : var -> var)
-         (n : nat)
-         (sl: ann (set var * set var * option (list (set var * set var ))))
-         {struct sl}
-  : ann (set var * set var * option (list (set var * set var)))
-  :=
-    let rm := snd (getAnn sl) in
-    (fix add_nones n
-        :=
-    match n with
-    | 0 =>
-        match sl with
-        | ann0 a => sl
-        | ann1 a sl_s
-          => ann1 a (do_spill_rm' slot (count sl_s) sl_s)
-        | ann2 a sl_s sl_t
-          => ann2 a (do_spill_rm' slot (count sl_s) sl_s)
-                    (do_spill_rm' slot (count sl_t) sl_t)
-        | annF a sl_F sl_t
-          => annF a ((fun sl_s => do_spill_rm' slot (count sl_s) sl_s) ⊝ sl_F)
-                    (do_spill_rm' slot (count   sl_t) sl_t)
-        end
-    | S n =>
-        ann1 (∅,∅,None) (add_nones n)
-    end) n
+Definition add_anns
+           (X : Type)
+           (an : X)
+           (n : nat)
+           (a : ann X)
+  : ann X
+  := iter n a (fun b => ann1 an b)
 .
 
+
+Lemma add_anns_S
+      (X : Type)
+      (an : X)
+      (n : nat)
+      (a : ann X)
+  :
+    add_anns an (S n) a = ann1 an (add_anns an n a)
+.
+Proof.
+  unfold add_anns.
+  general induction n;
+    simpl; eauto.
+Qed.
+
+Definition slot_merge
+           (slot : var -> var)
+  := List.map (fun (RM : set var * set var)
+               => fst RM ∪ map slot (snd RM))
+.
+
+
+
+Lemma slot_merge_app
+      (L1 L2: list (set var * set var))
+      (slot : var -> var)
+  :
+    slot_merge slot L1 ++ slot_merge slot L2
+      = slot_merge slot (L1 ++ L2)
+.
+Proof.
+  intros.
+  unfold slot_merge.
+  rewrite map_app; eauto.
+Qed.
+
+
+
+Fixpoint do_spill_rm
+         (slot : var -> var)
+         (sl : spilling)
+  : ann (option (list (⦃ var ⦄)))
+  :=
+    add_anns None (count sl)
+             (let rm' := option_map (slot_merge slot) (snd (getAnn sl)) in
+              match sl with
+              | ann0 _
+                => ann0 rm'
+
+              | ann1 _ sl0
+                => ann1 rm' (do_spill_rm slot sl0)
+
+              | ann2 _ sl1 sl2
+                => ann2 rm' (do_spill_rm slot sl1) (do_spill_rm slot sl2)
+
+              | annF _ slF sl2
+                => annF rm' (do_spill_rm slot ⊝ slF) (do_spill_rm slot sl2)
+              end
+             )
+.
+
+Lemma do_spill_rm_s
+      (slot : var -> var)
+      (sl : spilling)
+  :
+    do_spill_rm slot sl
+    = add_anns None (count sl) (do_spill_rm slot (setTopAnn sl (∅,∅,snd (getAnn sl))))
+.
+Proof.
+  unfold do_spill_rm.
+  destruct sl;
+    unfold count;
+    simpl;
+    rewrite empty_cardinal;
+    simpl;
+    eauto.
+Qed.
+
+
+(*
+
+Definition discard_merge_sl
+           (slot : var -> var)
+  : spilling -> ann (option (list (set var)))
+  :=
+    mapAnn (fun (a : set var * set var * option (list (set var * set var)))
+            => option_map (slot_merge slot) (snd a))
+.
+
+
+Fixpoint wrap_ann
+         (X : Type)
+         (wrap : ann X -> ann X)
+         (a : ann X)
+  : ann X
+  :=
+    wrap
+    match a with
+    | ann0 an => ann0 an
+    | ann1 an a1 => ann1 an (wrap_ann wrap a1)
+    | ann2 an a1 a2 => ann2 an (wrap_ann wrap a1) (wrap_ann wrap a2)
+    | annF an aF a1 => annF an (wrap_ann wrap ⊝ aF) (wrap_ann wrap a1)
+    end
+.
 
 
 Definition do_spill_rm
            (slot : var -> var)
-           (sl : ann (set var * set var * option (list (set var * set var))))
-  := do_spill_rm' slot (count sl) sl.
-
-
-
-Lemma do_spill_rm_s
-      (slot : var -> var)
-      (sl : ann (set var * set var * option (list (set var * set var))))
-      (n : nat)
-  :
-    do_spill_rm' slot (S n) sl
-    = ann1 (∅,∅,None) (do_spill_rm' slot n sl)
+           (sl : spilling)
+  : ann (option (list (set var)))
+  := discard_merge_sl slot
+                      (wrap_ann
+                         (fun sl => add_anns (∅,∅,None)
+                                           (count sl)
+                                            sl)
+                          sl)
 .
-Proof.
-  unfold do_spill_rm' at 1.
-  destruct sl;
-    simpl;
-    reflexivity.
-Qed.
-
 
 
 
@@ -65,20 +138,59 @@ Lemma do_spill_rm_zero
       (slot : var -> var)
       (sl : ann (set var * set var * option (list (set var * set var))))
   :
-    do_spill_rm' slot 0 sl
-    = match sl with
-       | ann0 (Sp, L, rm) => ann0 (Sp, L, rm)
-       | ann1 (Sp, L, rm) sl_s => ann1 (Sp, L, rm) (do_spill_rm slot sl_s)
-       | ann2 (Sp, L, rm) sl_s sl_t =>
-           ann2 (Sp, L, rm) (do_spill_rm slot sl_s) (do_spill_rm slot sl_t)
-       | annF (Sp, L, rm) sl_F sl_t =>
-           annF (Sp, L, rm) (do_spill_rm slot ⊝ sl_F) (do_spill_rm slot sl_t)
-       end
+    count sl = 0
+    -> do_spill_rm slot sl
+      = match sl with
+        | ann0 (_,rm)
+          => ann0 (option_map (slot_merge slot) rm)
+
+        | ann1 (_,rm) sl1
+          => ann1 (option_map (slot_merge slot) rm)
+                  (do_spill_rm slot sl1)
+
+        | ann2 (_,rm) sl1 sl2
+          => ann2 (option_map (slot_merge slot) rm)
+                  (do_spill_rm slot sl1)
+                  (do_spill_rm slot sl2)
+        | annF (_,rm) slF sl2
+          => annF (option_map (slot_merge slot) rm)
+                  ((do_spill_rm slot) ⊝ slF)
+                  ( do_spill_rm slot sl2)
+        end
 .
 Proof.
-  unfold do_spill_rm'.
-  induction sl; fold do_spill_rm';
+  intros count_zero.
+  destruct sl;
+    unfold do_spill_rm;
+    unfold discard_merge_sl;
+    unfold wrap_ann;
+    unfold count in *;
+    simpl in *;
+    rewrite count_zero;
+    simpl;
     destruct a;
     destruct p;
+    simpl;
+    try reflexivity.
+  fold wrap_ann.
+  enough (
+      (mapAnn (fun a : ⦃var⦄ * ⦃var⦄ * ؟ 〔⦃var⦄ * ⦃var⦄〕 => option_map (slot_merge slot) (snd a))
+      ⊝ wrap_ann
+          (fun sl0 : spilling => add_anns (∅, ∅, ⎣⎦) (cardinal (getSp sl0) + cardinal (getL sl0)) sl0)
+          ⊝ sa)
+      =
+      ((fun sl0 : spilling =>
+       mapAnn (fun a : ⦃var⦄ * ⦃var⦄ * ؟ 〔⦃var⦄ * ⦃var⦄〕 => option_map (slot_merge slot) (snd a))
+         (wrap_ann
+            (fun sl1 : spilling =>
+               add_anns (∅, ∅, ⎣⎦) (cardinal (getSp sl1) + cardinal (getL sl1)) sl1) sl0)) ⊝ sa)).
+  {
+    rewrite H.
     reflexivity.
+  }
+  induction sa; simpl; eauto.
+  f_equal.
+  apply IHsa.
 Qed.
+
+*)
