theories/Spilling/ReconstrLiveSound.v
@@ -1,0 +1,95 @@
+Require Import List Map Env AllInRel Exp AppExpFree.
+Require Import IL Annotation InRel AutoIndTac Liveness LabelsDefined.
+Require Import Spilling DoSpill DoSpillRm.
+Require Import SpillUtil ReconstrLive.
+
+Set Implicit Arguments.
+
+Lemma reconstr_live_sound_s
+      (slot : var -> var)
+      (ZL : list params)
+      (G M : set var)
+      (Λ : list (set var * set var))
+      (Lv : list (set var))
+      (s : stmt)
+      (sl : ann (set var * set var * option (list (set var * set var))))
+  :
+    let sl0 := setTopAnn sl (∅,∅,snd (getAnn sl)) in
+    (forall G' M', live_sound Imperative ZL Lv
+                     (do_spill slot M' s sl0)
+                     (reconstr_live (slot_merge slot Λ) ZL G'
+                                    (do_spill slot M' s sl0)
+                                    (do_spill_rm slot sl0)))
+   -> live_sound Imperative ZL Lv
+                (do_spill slot M s sl)
+                (reconstr_live (slot_merge slot Λ) ZL G
+                               (do_spill slot M s sl)
+                               (do_spill_rm slot sl)).
+Proof.
+  intros sl0 sls.
+  subst sl0.
+
+  rewrite do_spill_extract_writes.
+  rewrite do_spill_rm_s.
+
+  (* prepare induction *)
+  remember (elements (getSp sl)) as elSp.
+  remember (elements (getL  sl)) as elL.
+  assert (count sl = length elSp + length elL) as count_sl.
+  {
+    unfold count.
+    rewrite HeqelSp.
+    rewrite HeqelL.
+    do 2 rewrite elements_length.
+    reflexivity.
+  }
+  rewrite count_sl.
+  clear count_sl HeqelSp.
+  revert G M.
+  induction elSp;
+    intros G M;
+    fold do_spill.
+  - simpl.
+    revert G.
+    clear HeqelL.
+    induction elL;
+      intros G;
+      fold do_spill.
+    + simpl.
+      unfold add_anns.
+      simpl.
+      erewrite do_spill_Equal_M; eauto.
+      clear.
+      cset_tac.
+    + unfold length.
+      rewrite add_anns_S.
+      rewrite write_loads_s.
+      constructor; eauto; fold reconstr_live.
+      * simpl.
+        apply live_exp_sound_incl with (lv':=singleton (slot a)).
+        -- econstructor.
+           econstructor.
+           cset_tac.
+        -- clear.
+           cset_tac.
+      * clear.
+        cset_tac.
+      * apply reconstr_live_G.
+        cset_tac.
+  - replace (length (a::elSp) + length elL) with (S (length elSp + length elL))
+      by (simpl ; reflexivity).
+    rewrite add_anns_S.
+    rewrite write_spills_s.
+    constructor; eauto; fold reconstr_live.
+    * simpl.
+      apply live_exp_sound_incl with (lv':=singleton a).
+      -- econstructor.
+         econstructor.
+         cset_tac.
+      -- clear.
+         cset_tac.
+    * clear.
+      cset_tac.
+    * apply reconstr_live_G.
+      cset_tac.
+Qed.
