theories/Spilling/Spilling.v
@@ -2,91 +2,96 @@ Require Import List Map Env AllInRel Exp.
 Require Import IL Annotation InRel AutoIndTac Liveness LabelsDefined.
 Require Import SimI.
 
+Notation "'spilling'" := (ann (set var * set var * option (list (set var * set var)))).
+
+Notation "'getSp' sl" := (fst (fst (getAnn sl))) (at level 40).
+Notation "'getL' sl" := (snd (fst (getAnn sl))) (at level 40).
 
 Inductive spill_sound (k:nat) :
-(list params) ->
-(list (set var * set var)) ->
-(set var * set var) ->
-stmt ->
-ann (set var * set var * option (list (set var * set var)))
--> Prop :=
+  (list params)
+  -> (list (set var * set var))
+  -> (set var * set var)
+  -> stmt
+  -> spilling
+  -> Prop
+  :=
 
-| SpillLet ZL Λ R M Sp L K Kx sl x e s
-: Sp ⊆ R
-  -> L ⊆ Sp ∪ M
-  -> spill_sound k ZL Λ ({x;(R\K ∪ L)\Kx }, Sp ∪ M) s sl
-  -> Exp.freeVars e ⊆ R\K ∪ L
-  -> cardinal (R\K ∪ L) <= k
-  -> cardinal ({x;((R\K) ∪ L)\Kx }) <= k
-  -> spill_sound k ZL Λ (R,M) (stmtLet x e s) (ann1 (Sp,L,None) sl)
+  | SpillLet ZL Λ R M Sp L K Kx sl x e s
+    : Sp ⊆ R
+      -> L ⊆ Sp ∪ M
+      -> spill_sound k ZL Λ ({x;(R\K ∪ L)\Kx }, Sp ∪ M) s sl
+      -> Exp.freeVars e ⊆ R\K ∪ L
+      -> cardinal (R\K ∪ L) <= k
+      -> cardinal ({x;((R\K) ∪ L)\Kx }) <= k
+      -> spill_sound k ZL Λ (R,M) (stmtLet x e s) (ann1 (Sp,L,None) sl)
 
-| SpillReturn ZL Λ R M Sp L K e
-: Sp ⊆ R
-  -> L ⊆ Sp ∪ M
-  -> Op.freeVars e ⊆ R\K ∪ L
-  -> cardinal ((R\K) ∪ L) <= k
-  -> spill_sound k ZL Λ (R,M) (stmtReturn e) (ann0 (Sp,L,None))
+  | SpillReturn ZL Λ R M Sp L K e
+    : Sp ⊆ R
+      -> L ⊆ Sp ∪ M
+      -> Op.freeVars e ⊆ R\K ∪ L
+      -> cardinal ((R\K) ∪ L) <= k
+      -> spill_sound k ZL Λ (R,M) (stmtReturn e) (ann0 (Sp,L,None))
 
-| SpillIf ZL Λ R M Sp L K sl_s sl_t e s t
-: Sp ⊆ R
-  -> L ⊆ Sp ∪ M
-  -> Op.freeVars e ⊆ R\K ∪ L
-  -> cardinal (R\K ∪ L) <= k
-  -> spill_sound k ZL Λ (R\K ∪ L, Sp ∪ M) s sl_s
-  -> spill_sound k ZL Λ (R\K ∪ L, Sp ∪ M) t sl_t
-  -> spill_sound k ZL Λ (R,M) (stmtIf e s t) (ann2 (Sp,L,None) sl_s sl_t)
+  | SpillIf ZL Λ R M Sp L K sl_s sl_t e s t
+    : Sp ⊆ R
+      -> L ⊆ Sp ∪ M
+      -> Op.freeVars e ⊆ R\K ∪ L
+      -> cardinal (R\K ∪ L) <= k
+      -> spill_sound k ZL Λ (R\K ∪ L, Sp ∪ M) s sl_s
+      -> spill_sound k ZL Λ (R\K ∪ L, Sp ∪ M) t sl_t
+      -> spill_sound k ZL Λ (R,M) (stmtIf e s t) (ann2 (Sp,L,None) sl_s sl_t)
 
-| SpillApp ZL Z Λ R M Sp L K f Y R_f M_f
-: Sp ⊆ R
-  -> L ⊆ Sp ∪ M
-  -> cardinal (R\K ∪ L) <= k
-  (*-> list_union (Op.freeVars ⊝ Y) ⊆ R ∪ M*)
-  -> get ZL (counted f) Z
-  -> get Λ (counted f) (R_f,M_f)
-  -> R_f \ of_list Z ⊆ R\K ∪ L
-  -> M_f \ of_list Z ⊆ Sp ∪ M
-    -> spill_sound k ZL Λ (R,M) (stmtApp f Y) (ann0 (Sp,L,None))
+  | SpillApp ZL Z Λ R M Sp L K f Y R_f M_f
+    : Sp ⊆ R
+      -> L ⊆ Sp ∪ M
+      -> cardinal (R\K ∪ L) <= k
+      -> list_union (Op.freeVars ⊝ Y) ⊆ R ∪ M
+      -> get ZL (counted f) Z
+      -> get Λ (counted f) (R_f,M_f)
+      -> R_f \ of_list Z ⊆ R\K ∪ L
+      -> M_f \ of_list Z ⊆ Sp ∪ M
+      -> spill_sound k ZL Λ (R,M) (stmtApp f Y) (ann0 (Sp,L,None))
 
-| SpillFun (ZL:list params) Λ R M Sp L K t sl_F sl_t (F: list(params*stmt)) rms
-  : Sp ⊆ R
-  -> L ⊆ Sp ∪ M
-  -> cardinal (R\K ∪ L) <= k
-  -> length F = length sl_F
-  -> length F = length rms
-  -> (forall n rm, get rms n rm -> cardinal (fst rm) <= k)
-  -> (forall n Zs rm sl_s, get rms n rm
-     -> get F n Zs
-     -> get sl_F n sl_s
-     -> spill_sound k ((fst ⊝ F) ++ ZL) (rms ++ Λ) rm (snd Zs) sl_s
-     )
-  -> spill_sound k ((fst ⊝ F) ++ ZL) (rms ++ Λ) (R\K ∪ L, Sp ∪ M) t sl_t
-    -> spill_sound k ZL Λ (R,M) (stmtFun F t)
-                   (annF (Sp,L,Some rms) sl_F sl_t)
+  | SpillFun (ZL:list params) Λ R M Sp L K t sl_F sl_t (F: list(params*stmt)) rms
+    : Sp ⊆ R
+      -> L ⊆ Sp ∪ M
+      -> cardinal (R\K ∪ L) <= k
+      -> length F = length sl_F
+      -> length F = length rms
+      -> (forall n rm, get rms n rm -> cardinal (fst rm) <= k)
+      -> (forall n Zs rm sl_s, get rms n rm
+                         -> get F n Zs
+                         -> get sl_F n sl_s
+                         -> spill_sound k ((fst ⊝ F) ++ ZL) (rms ++ Λ) rm (snd Zs) sl_s
+        )
+      -> spill_sound k ((fst ⊝ F) ++ ZL) (rms ++ Λ) (R\K ∪ L, Sp ∪ M) t sl_t
+      -> spill_sound k ZL Λ (R,M) (stmtFun F t)
+                    (annF (Sp,L,Some rms) sl_F sl_t)
 .
 
 Inductive fv_e_bounded : nat -> stmt -> Prop :=
 
 | BoundLet k x e s
-: cardinal (Exp.freeVars e) <= k
-  -> fv_e_bounded k s
-  -> fv_e_bounded k (stmtLet x e s)
+  : cardinal (Exp.freeVars e) <= k
+    -> fv_e_bounded k s
+    -> fv_e_bounded k (stmtLet x e s)
 
 | BoundReturn k e
-: cardinal (Op.freeVars e) <= k
-  -> fv_e_bounded k (stmtReturn e)
+  : cardinal (Op.freeVars e) <= k
+    -> fv_e_bounded k (stmtReturn e)
 
 | BoundIf k e s t
-: cardinal (Op.freeVars e) <= k
-  -> fv_e_bounded k s
-  -> fv_e_bounded k t
-  -> fv_e_bounded k (stmtIf e s t)
+  : cardinal (Op.freeVars e) <= k
+    -> fv_e_bounded k s
+    -> fv_e_bounded k t
+    -> fv_e_bounded k (stmtIf e s t)
 
 | BoundApp k f Y
-: cardinal (list_union (Op.freeVars ⊝ Y)) <= k
-  -> fv_e_bounded k (stmtApp f Y)
+  : cardinal (list_union (Op.freeVars ⊝ Y)) <= k
+    -> fv_e_bounded k (stmtApp f Y)
 
 | BoundFun k F t
-: (forall n Zs, get F n Zs -> fv_e_bounded k (snd Zs))
-  -> fv_e_bounded k t
-  -> fv_e_bounded k (stmtFun F t)
+  : (forall n Zs, get F n Zs -> fv_e_bounded k (snd Zs))
+    -> fv_e_bounded k t
+    -> fv_e_bounded k (stmtFun F t)
 .
